array: re-write proof to directly encode and prove monotonicity

array-contains.bpl
@@ -5,257 +5,498 @@
 
 type Invoc;
 
-// Create an invocation. Methods are: 0 - put, 1 - get, 2 - contains
-function createInvoc(m: int, k: int, v: int) returns (i: Invoc);
+// function key(n: Invoc) returns (k: int);
+
+type Method;
+const unique get, put, contains: Method;
+
+// Create an invocation.
+function createInvoc(m: Method, k: int, v: int) returns (i: Invoc);
 
 
-type SeqInvoc;  // sequence of invocations
-
-
-function subseq(s: SeqInvoc, t: SeqInvoc) : bool;
-
-// subseq is reflexive
-axiom (forall s: SeqInvoc :: subseq(s, s));
-
-// subseq is transitive
-axiom (forall s, t, u: SeqInvoc :: subseq(s, t) && subseq(t, u) ==> subseq(s, u));
-
+// Sequences of invocations
+type SeqInvoc;
 
 function append(s: SeqInvoc, o: Invoc) returns (t: SeqInvoc);
 
-// append preserves subseq
-axiom (forall s, t: SeqInvoc, o: Invoc :: subseq(s, t) ==>
-        subseq(append(s, o), append(t, o)));
-axiom (forall s, t: SeqInvoc, o: Invoc :: subseq(s, t) ==>
-        subseq(s, append(t, o)));
+/*
+// append preserves subset
+axiom (forall s, t: SeqInvoc, o: Invoc :: subset(s, t) ==>
+        subset(append(s, o), append(t, o)));
+axiom (forall s, t: SeqInvoc, o: Invoc :: subset(s, t) ==>
+        subset(s, append(t, o)));
+*/
 
 
-function union(s1: SeqInvoc, s2: SeqInvoc) returns (t: SeqInvoc);
+// Sets of invocations -- TODO Z3 support?
+type SetInvoc;
+const emptySet: SetInvoc;
+
+// function elementOf(n: Invoc, s: SetInvoc) : bool;
+
+function subset(s: SetInvoc, t: SetInvoc) : bool;
+
+// emptySet is a subset of anything
+axiom (forall s: SetInvoc :: subset(emptySet, s));
+
+// subset is reflexive
+axiom (forall s: SetInvoc :: subset(s, s));
+
+// subset is transitive
+axiom (forall s, t, u: SetInvoc :: subset(s, t) && subset(t, u) ==> subset(s, u));
+
+function union(s1: SetInvoc, s2: SetInvoc) returns (t: SetInvoc);
 
 // union is idempotent
-axiom (forall s: SeqInvoc :: s == union(s, s));
+axiom (forall s: SetInvoc :: s == union(s, s));
 
 // union is associative
-axiom (forall s, t: SeqInvoc :: union(s, t) == union(t, s));
+axiom (forall s, t: SetInvoc :: union(s, t) == union(t, s));
 
-// union is monotonic w.r.t subseq
-axiom (forall s, t1, t2: SeqInvoc :: subseq(t1, t2) ==> subseq(union(s, t1), union(s, t2)));
+// union is monotonic w.r.t subset
+axiom (forall s, t1, t2: SetInvoc :: subset(t1, t2) ==> subset(union(s, t1), union(s, t2)));
 
+// Calculate the union of m[i] \cup ... \cup m[j-1]
+function unionRange(m: [int]SetInvoc, i: int, j: int) returns (s: SetInvoc);
 
-// A function to restrict a SeqInvoc to invocations involving key k
-function restr(s: SeqInvoc, k: int) returns (t: SeqInvoc);
+function setOfSeq(q: SeqInvoc) returns (s: SetInvoc);
 
-// restr is a subseq
-axiom (forall s: SeqInvoc, k: int :: subseq(restr(s, k), s));
+function add(s: SetInvoc, n: Invoc) returns (t: SetInvoc);
 
+// add preserves subset relation
+axiom (forall s, t: SetInvoc, n: Invoc :: subset(s, t) ==> subset(add(s, n), add(t, n)));
+axiom (forall s, t: SetInvoc, n: Invoc :: subset(s, t) ==> subset(s, add(t, n)));
 
-// A function to calculate the abstract state after a sequential execution
-function state(s: SeqInvoc) returns (m: [int]int);
+// Relation between setOfSeq, add, and append
+axiom (forall q: SeqInvoc, n: Invoc :: setOfSeq(append(q, n)) == add(setOfSeq(q), n));
+
+// Relation between unionRange, add, and append
+axiom (forall t: [int]SetInvoc, i, j, k: int, q: SeqInvoc, n: Invoc ::
+        unionRange(t, i, j) == setOfSeq(q) && i <= k && k < j ==>
+          unionRange(t[k := add(t[k], n)], i, j) == setOfSeq(append(q, n)));
+
+// Add n to m[i], ..., m[j-1]
+function addRange(m: [int]SetInvoc, n: Invoc, i: int, j: int)
+  returns (m1: [int]SetInvoc);
+
+// The effect of addRange
+axiom (forall m, m1: [int]SetInvoc, n: Invoc, i: int, j: int, k: int ::
+        m1 == addRange(m, n, i, j) && i <= k && k < j
+        ==> m1[k] == add(m[k], n));
+axiom (forall m, m1: [int]SetInvoc, n: Invoc, i: int, j: int, k: int ::
+        m1 == addRange(m, n, i, j) && !(i <= k && k < j)
+        ==> m1[k] == m[k]);
+
+// What happens to unionRange and setOfSeq when you do an addRange
+axiom (forall t: [int]SetInvoc, i, j, i1, j1: int, q: SeqInvoc, n: Invoc ::
+        unionRange(t, i, j) == setOfSeq(q) && i <= i1 && i1 < j1 && j1 <= j ==>
+          unionRange(addRange(t, n, i1, j1), i, j) == setOfSeq(append(q, n)));
+
+// A function to restrict a SetInvoc to invocations involving key k
+function restr(s: SetInvoc, k: int) returns (t: SetInvoc);
+
+// restr is a subset
+axiom (forall s: SetInvoc, k: int :: subset(restr(s, k), s));
+
+// restr is monotonic w.r.t subset
+axiom (forall s, t: SetInvoc, k: int :: subset(s, t) ==> subset(restr(s, k), restr(t, k)));
+
+// Adding an invocation on k increases restr
+axiom (forall q: SeqInvoc, n: Invoc, m: Method, k, v: int :: n == createInvoc(m, k, v) ==>
+        restr(setOfSeq(append(q, n)), k) == add(restr(setOfSeq(q), k), n)
+);
+
+// Adding invocations not on k preserves restr
+axiom (forall q: SeqInvoc, n: Invoc, m: Method, k, k1, v: int ::
+        n == createInvoc(m, k1, v) && k1 != k ==>
+        restr(setOfSeq(append(q, n)), k) == restr(setOfSeq(q), k)
+);
+
+type AbsState = [int]int; // Abstract state
+
+// A function to calculate the abstract state after executing a subset vis of
+// a sequence of invocations lin
+function state(vis: SetInvoc, lin: SeqInvoc) returns (m: AbsState);
 
 
 // ---------- Some lemmas of this ADT that we need
 
-// The mapping of key k depends only invocations involving k
-axiom (forall s: SeqInvoc, k: int :: state(s)[k] == state(restr(s, k))[k]);
+// The effect of appending an invocation on key k on state of k
+axiom (forall s1, s2: SetInvoc, q1, q2: SeqInvoc, n: Invoc, m: Method, k, v: int ::
+        n == createInvoc(m, k, v) && q2 == append(q1, n) && s2 == add(s1, n) ==>
+          (m == put ==> state(s2, q2)[k] == v)
+);
+axiom (forall s1, s2: SetInvoc, q1, q2: SeqInvoc, n: Invoc, m: Method, k, v: int ::
+        n == createInvoc(m, k, v) && q2 == append(q1, n) && s2 == add(s1, n) ==>
+          ((m == get || m == contains) ==> state(s2, q2)[k] == state(s1, q1)[k])
+);
+// TODO why doesn't this follow from the above?
+axiom (forall t1, t2: [int]SetInvoc, q1, q2: SeqInvoc, n: Invoc, i, j, k, k1, v: int ::
+        n == createInvoc(contains, k, v) && q2 == append(q1, n)
+        && t2 == addRange(t1, n, i, j) ==>
+          state(t2[k1], q2)[k1] == state(t1[k1], q1)[k1]
+);
 
+
+// The effect of appending an invocation on key k on state with unchanged vis
+axiom (forall s: SetInvoc, q1, q2: SeqInvoc, n: Invoc, m: Method, k, k1, v: int ::
+        n == createInvoc(m, k, v) && q2 == append(q1, n) ==>
+          state(s, q1)[k1] == state(s, q2)[k1]
+);
+
+
+// The mapping of key k depends only invocations involving k
+axiom (forall s: SetInvoc, q: SeqInvoc, k: int ::
+        state(s, q)[k] == state(restr(s, k), q)[k]);
+axiom (forall q: SeqInvoc, k: int ::
+        state(setOfSeq(q), q)[k] == state(restr(setOfSeq(q), k), q)[k]);
+
+// Taking union with a restriction of a super-set means restrictions are same
+axiom (forall s0, s1, t: SetInvoc, k: int ::
+        s1 == union(s0, t) && subset(restr(s0, k), t) ==>
+          restr(s1, k) == restr(t, k)
+);
+
+/*
 // Adding invocations of a key k does not affect state of keys k1 != k
 axiom (forall s, t: SeqInvoc, k, k1: int :: k != k1 ==>
         state(union(s, restr(t, k)))[k1] == state(s)[k1]);
 
-// The effect of appending an invocation on key k on state of other keys
-axiom (forall s1, s2: SeqInvoc, o: Invoc, m, k, v: int ::
-        s2 == append(s1, o) && o == createInvoc(m, k, v) ==>
-          (forall i: int :: i != k ==> state(s1)[i] == state(s2)[i])
-);
+*/
 
-// The effect of appending an invocation on key k on state of k
-axiom (forall s1, s2: SeqInvoc, o: Invoc, m, k, v: int ::
-        s2 == append(s1, o) && o == createInvoc(m, k, v) ==>
-          (m == 0 ==> state(s2)[k] == v)
-          && (m == 1 || m == 2 ==> state(s2)[k] == state(s1)[k])
-);
 
-// Taking union of a restriction of a super-sequence means restrictions are same
-axiom (forall s0, s1, t: SeqInvoc, k: int ::
-        s1 == union(s0, restr(t, k)) && subseq(s0, t) ==>
-          restr(s1, k) == restr(t, k)
-);
+// ---------- Representation of execution and linearization
 
+// A shared global variable that builds the linearization
+var {:layer 1,2} lin: SeqInvoc;
+
+// hb(x, y) : x happens-before y.
+// We assume there exists such a function, given by the client program
+function hb(x: Invoc, y: Invoc) : bool;
+
+// The set of invocations that have been called
+var {:layer 0,1} called: [Invoc]bool;
+
+// The set of invocations that have returned
+var {:layer 0,1} returned: [Invoc]bool;
+
+// A map from invocations to the set of prior invocations visible to them
+var vis: [Invoc]SetInvoc;
+
+// The invariants satisfied by the above
+function {:inline} linInv(lin: SeqInvoc, abs: AbsState, tabvis: [int]SetInvoc)
+  : bool
+{
+  (forall i: int :: 0 <= i && i < tableLen ==> state(tabvis[i], lin)[i] == abs[i])
+  && (forall i: int :: 0 <= i && i < tableLen ==>
+      state(tabvis[i], lin)[i] == state(restr(setOfSeq(lin), i), lin)[i])
+  && (forall i: int :: 0 <= i && i < tableLen ==> subset(restr(setOfSeq(lin), i), tabvis[i]))
+  // The linearization is consistent with happens-before
+}
 
 // ---------- Logical and concrete shared state
 
-// A shared global variable that builds the linearization
-var {:layer 0,2} lin: SeqInvoc;
+// Abstract state of ADT
+var {:layer 1,2} abs: AbsState;
+
+// Visibility per location of concrete state
+var {:layer 0,1} tabvis: [int]SetInvoc;
+
 
 // Concrete state of implementation
-var {:layer 0,2} table: [int]int;
+var {:layer 0,1} table: [int]int;
 const tableLen: int;
 axiom 0 <= tableLen;
 
-// Invariant
-function {:inline} tableInv(table: [int]int, lin: SeqInvoc) : bool
+
+function {:inline} abstracts(conc: [int]int, abs: AbsState) : bool
 {
-  (forall i: int :: 0 <= i && i < tableLen ==> table[i] == state(lin)[i])
+  (forall i: int :: 0 <= i && i < tableLen ==> conc[i] == abs[i])
+}
+
+// Invariant
+function {:inline} tableInv(table: [int]int, abs: AbsState, tabvis: [int]SetInvoc,
+                            lin: SeqInvoc) : bool
+{
+  abstracts(table, abs)
+  && unionRange(tabvis, 0, tableLen) == setOfSeq(lin)
+  && linInv(lin, abs, tabvis)
 }
 
 
 // ---------- Primitives/helpers for modifying global state
 
-procedure {:atomic} {:layer 1} writeTable_spec(k, v: int)
-  modifies table, lin;
+// Write to the table and returns the union of tabvis as the visibility
+procedure {:atomic} {:layer 1} writeTable_spec(k, v: int, n: Invoc)
+  returns (my_vis: SetInvoc, old_tabvis: [int]SetInvoc)
+  modifies table, vis, tabvis;
 {
+  old_tabvis := tabvis;
   table[k] := v;
-  lin := append(lin, createInvoc(0, k, v));
-}
-procedure {:yields} {:layer 0} {:refines "writeTable_spec"} writeTable(k, v: int);
 
-procedure {:atomic} {:layer 1} readTable_spec(k: int) returns (v: int)
-  modifies lin;
+  tabvis[k] := add(tabvis[k], n);
+  assume my_vis == unionRange(tabvis, 0, tableLen);
+  vis[n] := my_vis;
+}
+procedure {:yields} {:layer 0} {:refines "writeTable_spec"}
+  writeTable(k, v: int, n: Invoc) returns (my_vis: SetInvoc, old_tabvis: [int]SetInvoc);
+
+// Read from the table and returns the union of tabvis as the visibility
+procedure {:atomic} {:layer 1} readTable_spec(k: int, n: Invoc)
+  returns (v: int, my_vis: SetInvoc)
+  modifies vis, tabvis;
 {
   v := table[k];
-  lin := append(lin, createInvoc(1, k, v));
-}
-procedure {:yields} {:layer 0} {:refines "readTable_spec"} readTable(k: int)
-  returns (v: int);
 
-procedure {:atomic} {:layer 1} copy_lin_spec() returns (s: SeqInvoc)
-{
-  s := lin;
+  tabvis[k] := add(tabvis[k], n);
+  assume my_vis == unionRange(tabvis, 0, tableLen);
+  vis[n] := my_vis;
 }
-procedure {:yields} {:layer 0} {:refines "copy_lin_spec"} copy_lin()
-  returns (s: SeqInvoc);
+procedure {:yields} {:layer 0} {:refines "readTable_spec"} readTable(k: int, n: Invoc)
+  returns (v: int, my_vis: SetInvoc);
 
-procedure {:atomic} {:layer 1} readTable1_spec(k: int, vis: SeqInvoc)
-  returns (v: int, old_vis, new_vis: SeqInvoc)
+
+// Read from the table and add the tabvis entry to the visibility
+procedure {:atomic} {:layer 1} readTable1_spec(k: int, my_vis: SetInvoc)
+  returns (v: int, old_vis, new_vis: SetInvoc)
 {
   v := table[k];
-  old_vis := vis;
-  new_vis := union(vis, restr(lin, k));
+
+  old_vis := my_vis;
+  new_vis := union(my_vis, tabvis[k]);
 }
 procedure {:yields} {:layer 0} {:refines "readTable1_spec"}
-  readTable1(k: int, vis: SeqInvoc) returns (v: int, old_vis, new_vis: SeqInvoc);
+  readTable1(k: int, my_vis: SetInvoc) returns (v: int, old_vis, new_vis: SetInvoc);
 
-procedure {:atomic} {:layer 1} linearizeC_spec(k, v: int)
+
+// Write my_vis to vis, and also add my label n to all of tabvis[]  -- TODO rename
+procedure {:atomic} {:layer 1} addVis_spec(n: Invoc, my_vis: SetInvoc, i: int)
+  returns (old_tabvis: [int]SetInvoc)
+  modifies vis, tabvis;
+{
+  old_tabvis := tabvis;
+  vis[n] := my_vis;
+  tabvis := addRange(tabvis, n, 0, i+1);
+}
+procedure {:yields} {:layer 0} {:refines "addVis_spec"}
+  addVis(n: Invoc, my_vis: SetInvoc, i: int)  returns (old_tabvis: [int]SetInvoc);
+
+
+// Introduction actions:
+
+procedure {:layer 1} {:inline 1} intro_writeLin1(n: Invoc) returns (old_lin: SeqInvoc)
   modifies lin;
 {
-  lin := append(lin, createInvoc(2, k, v));
+  old_lin := lin;
+  lin := append(lin, n);
 }
-procedure {:yields} {:layer 0} {:refines "linearizeC_spec"}
-  linearizeC(k, v: int);
+
+procedure {:layer 1} {:inline 1} intro_writeLin(n: Invoc)
+  modifies lin;
+{
+  lin := append(lin, n);
+}
+
+procedure {:layer 1} {:inline 1} intro_writeAbs(k: int, v: int)
+  modifies abs;
+{
+  abs[k] := v;
+}
+
+// Special call and return actions
+
+procedure {:atomic} {:layer 1} spec_call_spec(n: Invoc)
+  modifies called;
+{
+  called[n] := true;
+}
+procedure {:yields} {:layer 0} {:refines "spec_call_spec"} spec_call(n: Invoc);
+
+procedure {:atomic} {:layer 1} spec_return_spec(n: Invoc)
+  modifies returned;
+{
+  returned[n] := true;
+}
+procedure {:yields} {:layer 0} {:refines "spec_return_spec"}  spec_return(n: Invoc);
 
 
 // ---------- The ADT methods
 
 procedure {:atomic} {:layer 2} put_spec(k: int, v: int)
-  modifies table, lin;
+  returns (my_vis: SetInvoc)
+  modifies abs, lin, vis;
 {
-  table[k] := v;
-  lin := append(lin, createInvoc(0, k, v));
+  var this: Invoc;
+  this := createInvoc(put, k, v);
+  lin := append(lin, this);
+  vis := vis[this := my_vis];
+  // Put is complete
+  assume my_vis == setOfSeq(lin);
+
+  // Put satisfies its functional spec
+  abs[k] := v;
 }
 
-procedure {:yields} {:layer 1} {:refines "put_spec"}  put(k, v: int)
-  requires {:layer 1} tableInv(table, lin);
-  ensures {:layer 1} tableInv(table, lin);
+procedure {:yields} {:layer 1} {:refines "put_spec"} put(k, v: int)
+  returns (my_vis: SetInvoc)
+  requires {:layer 1} tableInv(table, abs, tabvis, lin);
+  requires {:layer 1} 0 <= k && k < tableLen;
+  ensures {:layer 1} tableInv(table, abs, tabvis, lin);
 {
-  yield; assert {:layer 1} tableInv(table, lin);
+  var this: Invoc; var old_tabvis: [int]SetInvoc;
+  this := createInvoc(put, k, v);
+  yield; assert {:layer 1} tableInv(table, abs, tabvis, lin);
+  call spec_call(this);
+  yield; assert {:layer 1} tableInv(table, abs, tabvis, lin);
 
-  call writeTable(k, v);
+  call my_vis, old_tabvis := writeTable(k, v, this);
 
-  yield; assert {:layer 1} tableInv(table, lin);
+  call intro_writeAbs(k, v);
+  call intro_writeLin(this);
+
+  yield; assert {:layer 1} tableInv(table, abs, tabvis, lin);
+  call spec_return(this);
+  yield; assert {:layer 1} tableInv(table, abs, tabvis, lin);
+}
+
+procedure {:atomic} {:layer 2} get_spec(k: int) returns (v: int, my_vis: SetInvoc)
+  modifies lin, vis;
+{
+  var this: Invoc;
+  this := createInvoc(get, k, v);
+  lin := append(lin, this);
+  vis := vis[this := my_vis];
+  // Get is complete -- TODO make predicate
+  assume my_vis == setOfSeq(lin);
+
+  // Get satisfies its functional spec
+  v := abs[k];
+}
+
+procedure {:yields} {:layer 1} {:refines "get_spec"} get(k: int)
+  returns (v: int, my_vis: SetInvoc)
+  requires {:layer 1} tableInv(table, abs, tabvis, lin);
+  requires {:layer 1} 0 <= k && k < tableLen;
+  ensures {:layer 1} tableInv(table, abs, tabvis, lin);
+{
+  var this: Invoc;
+  this := createInvoc(get, k, v);
+  yield; assert {:layer 1} tableInv(table, abs, tabvis, lin);
+  call spec_call(this);
+  yield; assert {:layer 1} tableInv(table, abs, tabvis, lin);
+
+  call v, my_vis := readTable(k, this);
+
+  call intro_writeLin(this);
+
+  yield; assert {:layer 1} tableInv(table, abs, tabvis, lin);
+  call spec_return(this);
+  yield; assert {:layer 1} tableInv(table, abs, tabvis, lin);
 }
 
 
-procedure {:atomic} {:layer 2} get_spec(k: int) returns (v: int)
-  modifies lin;
+function contains_func_spec(vis: SetInvoc, lin: SeqInvoc, witness_k: int,
+                            v: int, res: bool) : bool
 {
-  v := table[k];
-  lin := append(lin, createInvoc(1, k, v));
-}
-
-procedure {:yields} {:layer 1} {:refines "get_spec"} get(k: int) returns (v: int)
-  requires {:layer 1} tableInv(table, lin);
-  ensures {:layer 1} tableInv(table, lin);
-{
-  yield; assert {:layer 1} tableInv(table, lin);
-
-  call v := readTable(k);
-
-  yield; assert {:layer 1} tableInv(table, lin);
-}
-
-function contains_func_spec(s: SeqInvoc, witness_k: int, v: int, res: bool)
-  : bool
-{
-   (res ==> state(s)[witness_k] == v)
-   && (!res ==> (forall i: int :: 0 <= i && i < tableLen ==> state(s)[i] != v))
+   (res ==> state(vis, lin)[witness_k] == v)
+   && (!res ==> (forall i: int :: 0 <= i && i < tableLen ==> state(vis, lin)[i] != v))
 }
 
 procedure {:atomic} {:layer 2} contains_spec(v: int)
-  returns (res: bool, vis: SeqInvoc, witness_k: int)
-  modifies lin;
+  returns (res: bool, my_vis: SetInvoc, witness_k: int)
+  modifies lin, vis;
 {
-  lin := append(lin, createInvoc(2, witness_k, v));
-  assume subseq(vis, lin);
-  assume contains_func_spec(vis, witness_k, v, res);
+  var this: Invoc;
+  this := createInvoc(contains, witness_k, v);
+  lin := append(lin, createInvoc(contains, witness_k, v));
+  vis := vis[this := my_vis];
+  // Contains is monotonic
+  assume (forall j: Invoc :: hb(j, this) ==> subset(vis[j], my_vis));
+
+  // Contains satisfies its functional spec
+  assume contains_func_spec(my_vis, lin, witness_k, v, res);
 }
 
 procedure {:yields} {:layer 1} {:refines "contains_spec"} contains(v: int)
-  returns (res: bool, vis: SeqInvoc, witness_k: int)
-  requires {:layer 1} tableInv(table, lin);
-  ensures {:layer 1} tableInv(table, lin);
+  returns (res: bool, my_vis: SetInvoc, witness_k: int)
+  requires {:layer 1} tableInv(table, abs, tabvis, lin);
+  ensures {:layer 1} tableInv(table, abs, tabvis, lin);
 {
   var k, tv: int;
-  var old_vis: SeqInvoc;
+  var old_vis: SetInvoc;
+  var this: Invoc;
+  var old_tabvis: [int]SetInvoc; var {:layer 1} old_lin: SeqInvoc;
 
-  yield; assert {:layer 1} tableInv(table, lin);
-  call vis := copy_lin();
-
-  yield; assert {:layer 1} subseq(vis, lin) && tableInv(table, lin);
+  yield; assert {:layer 1} tableInv(table, abs, tabvis, lin);
   k := 0;
+  my_vis := emptySet;
   while (k < tableLen)
     invariant {:layer 1} 0 <= k && k <= tableLen;
-    invariant {:layer 1} subseq(vis, lin);
-    invariant {:layer 1} (forall i: int :: 0 <= i && i < k ==> state(vis)[i] != v);
-    invariant {:layer 1} tableInv(table, lin);
+    invariant {:layer 1} (forall i: int :: 0 <= i && i < k ==> state(my_vis, lin)[i] != v);
+    invariant {:layer 1} subset(my_vis, setOfSeq(lin));
+    invariant {:layer 1} tableInv(table, abs, tabvis, lin);
   {
-    // Read table[k] and add restr(lin, k) to vis
-    call tv, old_vis, vis := readTable1(k, vis);
+    // Read table[k] and add tabvis[k] to my_vis
+    call tv, old_vis, my_vis := readTable1(k, my_vis);
 
-    // tv == table[k] == state(lin)[k] == state(restr(lin, k))[k]
-    // == state(restr(vis, k))[k] == state(vis)[k]
-    assert {:layer 1} state(restr(lin, k))[k] == state(restr(vis, k))[k];
-    assert {:layer 1} tv == state(vis)[k];
-    // also, restr(lin, k) subseq lin ==> vis subseq lin
-    assert {:layer 1} subseq(union(old_vis, restr(lin, k)), union(old_vis, lin));
-    assert {:layer 1} subseq(union(old_vis, lin), union(lin, lin));
-    assert {:layer 1} subseq(vis, lin);
-
-    yield; assert {:layer 1} subseq(vis, lin) && tableInv(table, lin);
+    // tv == table[k] == abs[k] == state(tabvis[k], lin)[k]
+    // old_vis < setOfSeq(lin) ==> restr(old_vis, k) < restr(setOfSeq(lin), k)
+    assert {:layer 1} subset(restr(old_vis, k), restr(setOfSeq(lin), k));
+    // linInv() ==> restr(setOfSeq(lin), k) < tabvis[k]
+    // axiom ==> restr(my_vis, k) == restr(tabvis[k], k)
+    assert {:layer 1} state(restr(my_vis, k), lin)[k]
+                        == state(restr(tabvis[k], k), lin)[k];
+    // == tv
+    yield; assert {:layer 1} tableInv(table, abs, tabvis, lin) && tv == state(my_vis, lin)[k];
 
     if (tv == v) {
       // Linearization point
-      vis := append(vis, createInvoc(2, k, v));
+      this := createInvoc(contains, k, v);
+      my_vis := add(my_vis, this);
       witness_k := k;
-      call linearizeC(k, v);
+      call old_tabvis := addVis(this, my_vis, k);
+      call old_lin := intro_writeLin1(this);
 
       res := true;
 
-      yield; assert {:layer 1} subseq(vis, lin) && tableInv(table, lin);
+      assert {:layer 1} (forall i: int :: 0 <= i && i < tableLen ==>
+                           state(tabvis[i], lin)[i] == abs[i]);
+      assert {:layer 1} (forall i: int :: k < i && i < tableLen ==>
+                           subset(restr(setOfSeq(lin), i), tabvis[i]));
+      assert {:layer 1} (forall i: int :: 0 <= i && i < k ==>
+                           restr(setOfSeq(lin), i) == restr(setOfSeq(old_lin), i)
+                           && tabvis[i] == add(old_tabvis[i], this));
+      assert {:layer 1} (forall i: int :: 0 <= i && i < k ==>
+                           restr(setOfSeq(lin), i) == restr(setOfSeq(old_lin), i));
+      assert {:layer 1} (restr(setOfSeq(lin), k)
+                            == add(restr(setOfSeq(old_lin), k), this)
+                          && tabvis[k] == add(old_tabvis[k], this));
+      assert {:layer 1} (subset(restr(setOfSeq(lin), k), tabvis[k]));
+
+      // CONTINUE here: need to prove monotonicity
+      yield; assert {:layer 1} tableInv(table, abs, tabvis, lin);
       return;
     }
-    yield; assert {:layer 1} subseq(vis, lin) && tableInv(table, lin);
+    yield; assert {:layer 1} tableInv(table, abs, tabvis, lin);
 
     k := k + 1;
   }
-  yield; assert {:layer 1} subseq(vis, lin) && tableInv(table, lin);
+  yield; assert {:layer 1} tableInv(table, abs, tabvis, lin);
 
   // Linearization point
-  vis := append(vis, createInvoc(2, k, v));
+  this := createInvoc(contains, k, v);
+  my_vis := add(my_vis, this);
   witness_k := k;
-  call linearizeC(k, v);
+  call old_tabvis := addVis(this, my_vis, k-1);
+  call old_lin := intro_writeLin1(this);
 
   res := false;
 
-  yield; assert {:layer 1} tableInv(table, lin);
+  yield; assert {:layer 1} tableInv(table, abs, tabvis, lin);
   return;
 }
+
+
+// How to create a constant map with a default value, using a Z3 builtin
+// function {:builtin "MapConst"} createMapConst(bool) : [Invoc]bool;
+
